theories/DSub/adequacy.v
@@ -1,0 +1,44 @@
+From iris.program_logic Require Import adequacy.
+From iris.proofmode Require Import tactics.
+From D Require Import tactics.
+From D.DSub Require Import unary_lr.
+
+From iris.base_logic.lib Require Import gen_heap.
+
+Theorem adequacy Σ `{HdsubG: dsubPreG Σ} e e' thp σ σ' T ρ:
+  (forall `{dsubG Σ}, True ⊢ ⟦ T ⟧ₑ ρ e) →
+  rtc erased_step ([e], σ) (thp, σ') → e' ∈ thp →
+  is_Some (to_val e') ∨ reducible e' σ'.
+Proof.
+  intros Hlog ??. cut (adequate NotStuck e σ (λ _ _, True)); first (intros [_ ?]; eauto).
+  eapply (wp_adequacy Σ); eauto. apply HdsubG.
+  iIntros (Hinv ?). iModIntro. iExists (λ _ _, True%I). iSplit=> //.
+  (* rewrite -(empty_env_subst e). *)
+  (* Works: *)
+  (* iMod (gen_heap_init ∅) as "H". *)
+  (* iDestruct "H" as (g) "H1". *)
+  Fail iMod (gen_heap_init ∅) as (g) "H".
+
+  iMod (@gen_heap_init _ _ _ _ _ dsubPreG_interpNames ∅) as (g) "H".
+  set (DsubΣ := DsubG Σ Hinv _ g).
+  iApply (wp_wand with "[]"); by [iApply Hlog | auto].
+Qed.
+
+(* Instead of still assuming semantic typing, here we should assume syntactic
+   typing and use the fundamental lemma. But otherwise this follows the general
+   instantiation pattern, from e.g.
+   https://gitlab.mpi-sws.org/iris/examples/blob/a89dc12821b63eeb9b831d21629ac55ebd601f38/theories/logrel/F_mu_ref/soundness.v#L29-39. *)
+Corollary almost_type_soundness e e' thp σ σ' T:
+  (forall `{dsubG Σ}, True ⊢ ⟦ T ⟧ₑ [] e) →
+  rtc erased_step ([e], σ) (thp, σ') → e' ∈ thp →
+  is_Some (to_val e') ∨ reducible e' σ'.
+Proof.
+  intros ??. set (Σ := dsubΣ).
+  (* set (HG := DsubPreG Σ _ (subG_savedAnythingΣ _)). *)
+  set (HG := _: dsubPreG Σ).
+  eapply (adequacy Σ).
+  - intros ?.
+    apply H.
+      (* by apply fundamental. *)
+  - eauto.
+Qed.
